Simplified the proofs of an old entry

thys/BinarySearchTree/BinaryTree_Map.thy
@@ -23,13 +23,13 @@ type_synonym
   'a tarray = "(index * 'a) Tree"
 
 definition valid_tmap :: "'a tarray => bool" where
-  "valid_tmap t == sortedTree fst t"
+  "valid_tmap t \<equiv> sortedTree fst t"
 
 declare valid_tmap_def [simp]
 
 definition mapOf :: "'a tarray => index => 'a option" where
   \<comment> \<open>the abstraction function from trees to maps\<close>
-  "mapOf t i == 
+  "mapOf t i \<equiv>
    (case (tlookup fst i t) of
      None => None
    | Some ia => Some (snd ia))"
@@ -39,109 +39,65 @@ section \<open>Auxiliary Properties of our Implementation\<close>
 (*============================================================*)
 
 lemma mapOf_lookup1: "tlookup fst i t = None ==> mapOf t i = None"
-by (simp add: mapOf_def)
+  by (simp add: mapOf_def)
 
 lemma mapOf_lookup2: "tlookup fst i t = Some (j,a) ==> mapOf t i = Some a"
-by (simp add: mapOf_def)
+  by (simp add: mapOf_def)
 
-lemma assumes h: "mapOf t i = None"
-      shows mapOf_lookup3: "tlookup fst i t = None"
+lemma mapOf_lookup3: 
+    assumes h: "mapOf t i = None"
+    shows "tlookup fst i t = None"
 proof (cases "tlookup fst i t")
-case None from this show ?thesis by assumption
-next case (Some ia) note tsome = this
-  from this have o1: "tlookup fst i t = Some (fst ia, snd ia)" by simp
-  have "mapOf t i = Some (snd ia)"
-  by (insert mapOf_lookup2 [of i t "fst ia" "snd ia"], simp add: o1)
-  from this have "mapOf t i ~= None" by simp
-  from this h show ?thesis by simp \<comment> \<open>contradiction\<close>
+  case None 
+  then show ?thesis by assumption
+next 
+  case (Some ia) 
+  then show ?thesis
+    by (metis h mapOf_def option.discI option.simps(5))
 qed
 
-lemma assumes v: "valid_tmap t"
-      assumes h: "mapOf t i = Some a"
-      shows mapOf_lookup4: "tlookup fst i t = Some (i,a)"
+lemma mapOf_lookup4: 
+  assumes v: "valid_tmap t"
+  assumes h: "mapOf t i = Some a"
+  shows "tlookup fst i t = Some (i,a)"
 proof (cases "tlookup fst i t")
-case None 
-  from this mapOf_lookup1 have "mapOf t i = None" by auto
-  from this h show ?thesis by simp \<comment> \<open>contradiction\<close>
-next case (Some ia) note tsome = this
-  have tlookup_some_inst: "sortedTree fst t & (tlookup fst i t = Some ia) --> 
-        ia : setOf t & fst ia = i" by (simp add: tlookup_some)
-  from tlookup_some_inst tsome v have "ia : setOf t" by simp
-  from tsome have "mapOf t i = Some (snd ia)" by (simp add: mapOf_def)
-  from this h have o1: "snd ia = a" by simp
-  from tlookup_some_inst tsome v have o2: "fst ia = i" by simp
-  from o1 o2 have "ia = (i,a)" by auto
-  from this tsome show "tlookup fst i t = Some (i, a)" by simp
+  case None 
+  then show ?thesis
+    by (metis h mapOf_lookup1 option.discI)
+next 
+  case (Some ia) 
+  then show ?thesis
+    by (metis h mapOf_def option.simps(5) prod.exhaust_sel tlookup_some v
+        valid_tmap_def)
 qed
 
 subsection \<open>Lemmas \<open>mapset_none\<close> and \<open>mapset_some\<close> establish 
               a relation between the set and map abstraction of the tree\<close>
 
-lemma assumes v: "valid_tmap t"
-      shows mapset_none: "(mapOf t i = None) = (\<forall>a. (i,a) \<notin> setOf t)"
-proof
-  \<comment> \<open>==>\<close>
-  assume mapNone: "mapOf t i = None"
-  from v mapNone mapOf_lookup3 have lnone: "tlookup fst i t = None" by auto
-  show "\<forall>a. (i,a) \<notin> setOf t"
-  proof
-    fix a
-    show "(i,a) ~: setOf t"
-    proof
-      assume iain: "(i,a) : setOf t"
-      have tlookup_none_inst: 
-      "sortedTree fst t & (tlookup fst i t = None) --> (\<forall>x \<in> setOf t. fst x ~= i)"
-      by (insert tlookup_none [of "fst" "t" "i"], assumption)
-      from v lnone tlookup_none_inst have "\<forall>x \<in> setOf t. fst x ~= i" by simp
-      from this iain have "fst (i,a) ~= i" by fastforce
-      from this show False by simp
-    qed
-  qed
-  \<comment> \<open><==\<close>
-  next assume h: "\<forall>a. (i,a) \<notin> setOf t"
-  show "mapOf t i = None"
-  proof (cases "mapOf t i")
-  case None then show ?thesis .
-  next case (Some a) note mapsome = this
-    from v mapsome have o1: "tlookup fst i t = Some (i,a)" by (simp add: mapOf_lookup4)
-    (* moving mapOf_lookup4 to assumption does not work, although it uses
-       no == !! *)
-    from tlookup_some have tlookup_some_inst:
-    "sortedTree fst t & tlookup fst i t = Some (i,a) --> 
-     (i,a) : setOf t & fst (i,a) = i"
-    by (insert tlookup_some [of fst t i "(i,a)"], assumption)   
-    from v o1 this have "(i,a) : setOf t" by simp
-    from this h show ?thesis by auto \<comment> \<open>contradiction\<close>
-  qed
-qed
+lemma mapset_none: 
+  assumes "valid_tmap t"
+  shows "(mapOf t i = None) = (\<forall>a. (i,a) \<notin> setOf t)"
+  using assms 
+  unfolding valid_tmap_def
+  by (metis mapOf_lookup1 mapOf_lookup3 not_None_eq split_pairs tlookup_none
+      tlookup_some)
 
-lemma assumes v: "valid_tmap t"
-      shows mapset_some: "(mapOf t i = Some a) = ((i,a) : setOf t)"
-proof
-  \<comment> \<open>==>\<close>
-  assume mapsome: "mapOf t i = Some a"
-  from v mapsome have o1: "tlookup fst i t = Some (i,a)" by (simp add: mapOf_lookup4)
-  from tlookup_some have tlookup_some_inst:
-  "sortedTree fst t & tlookup fst i t = Some (i,a) --> 
-   (i,a) : setOf t & fst (i,a) = i"
-  by (insert tlookup_some [of fst t i "(i,a)"], assumption)   
-  from v o1 this show "(i,a) : setOf t" by simp
-  \<comment> \<open><==\<close>
-  next assume iain: "(i,a) : setOf t"
-  from v iain tlookup_finds have "tlookup fst (fst (i,a)) t = Some (i,a)" by fastforce
-  from this have "tlookup fst i t = Some (i,a)" by simp
-  from this show "mapOf t i = Some a" by (simp add: mapOf_def)
-qed
+lemma mapset_some: 
+  assumes "valid_tmap t"
+  shows "(mapOf t i = Some a) = ((i,a) \<in> setOf t)"
+  unfolding valid_tmap_def
+  using assms mapOf_lookup2 mapOf_lookup4 tlookup_finds tlookup_some
+  by fastforce
 
 (*============================================================*)
 section \<open>Empty Map\<close>
 (*============================================================*)
 
 lemma mnew_spec_valid: "valid_tmap Tip"
-by (simp add: mapOf_def)
+  by (simp add: mapOf_def)
 
 lemma mtip_spec_empty: "mapOf Tip k = None"
-by (simp add: mapOf_def)
+  by (simp add: mapOf_def)
 
 
 (*============================================================*)
@@ -149,111 +105,69 @@ section \<open>Map Update Operation\<close>
 (*============================================================*)
 
 definition mupdate :: "index => 'a => 'a tarray => 'a tarray" where
-  "mupdate i a t == binsert fst (i,a) t"
+  "mupdate i a t \<equiv> binsert fst (i,a) t"
 
-lemma assumes v: "valid_tmap t"
-      shows mupdate_map: "mapOf (mupdate i a t) = (mapOf t)(i |-> a)"
+lemma  mupdate_map:
+  assumes "valid_tmap t"
+  shows "mapOf (mupdate i a t) = (mapOf t)(i |-> a)"
 proof
-  fix i2
+  fix j
   let ?tr = "binsert fst (i,a) t"
   have upres: "mupdate i a t = ?tr" by (simp add: mupdate_def)
-  from v binsert_set 
-  have setSpec: "setOf ?tr = setOf t - eqs fst (i,a) Un {(i,a)}" by fastforce
-  from v binsert_sorted have vr: "valid_tmap ?tr" by fastforce
-  show "mapOf (mupdate i a t) i2 = ((mapOf t)(i |-> a)) i2"
-  proof (cases "i = i2")
-  case True note i2ei = this
-    from i2ei have rhs_res: "((mapOf t)(i |-> a)) i2 = Some a" by simp
-    have lhs_res: "mapOf (mupdate i a t) i = Some a"
-    proof -
-      have will_find: "tlookup fst i ?tr = Some (i,a)"
-      proof -
-        from setSpec have kvin: "(i,a) : setOf ?tr" by simp
-        have binsert_sorted_inst: "sortedTree fst t --> 
-                                 sortedTree fst ?tr"
-        by (insert binsert_sorted [of "fst" "t" "(i,a)"], assumption)
-        from v binsert_sorted_inst have rs: "sortedTree fst ?tr" by simp
-        have tlookup_finds_inst: "sortedTree fst ?tr & (i,a) : setOf ?tr --> 
-                                  tlookup fst i ?tr = Some (i,a)"
-        by (insert tlookup_finds [of "fst" "?tr" "(i,a)"], simp)
-        from rs kvin tlookup_finds_inst show ?thesis by simp
-      qed
-      from upres will_find show ?thesis by (simp add: mapOf_def)
-    qed
-    from lhs_res rhs_res i2ei show ?thesis by simp
-  next case False note i2nei = this
-    from i2nei have rhs_res: "((mapOf t)(i |-> a)) i2 = mapOf t i2" by auto
-    have lhs_res: "mapOf (mupdate i a t) i2 = mapOf t i2"
-    proof (cases "mapOf t i2")
-    case None from this have mapNone: "mapOf t i2 = None" by simp
-      from v mapNone mapset_none have i2nin: "\<forall>a. (i2,a) \<notin> setOf t" by fastforce
-      have noneIn: "\<forall>b. (i2,b) \<notin> setOf ?tr"
-      proof 
-        fix b 
-        from v binsert_set 
-        have "setOf ?tr = setOf t - eqs fst (i,a) Un {(i,a)}"
-        by fastforce
-        from this i2nei i2nin show "(i2,b) ~: setOf ?tr" by fastforce
-      qed
-      have mapset_none_inst: 
-      "valid_tmap ?tr --> (mapOf ?tr i2 = None) = (\<forall>a. (i2, a) \<notin> setOf ?tr)" 
-      by (insert mapset_none [of "?tr" i2], simp)
-      from vr noneIn mapset_none_inst have "mapOf ?tr i2 = None" by fastforce
-      from this upres mapNone show ?thesis by simp
-    next case (Some z) from this have mapSome: "mapOf t i2 = Some z" by simp
-      from v mapSome mapset_some have "(i2,z) : setOf t" by fastforce
-      from this setSpec i2nei have "(i2,z) : setOf ?tr" by (simp add: eqs_def)
-      from this vr mapset_some have "mapOf ?tr i2 = Some z" by fastforce
-      from this upres mapSome show ?thesis by simp
+  from assms binsert_set 
+  have setSpec: "setOf ?tr = setOf t - eqs fst (i,a) Un {(i,a)}" 
+    by fastforce
+  from assms binsert_sorted have vr: "valid_tmap ?tr" 
+    by fastforce
+  show "mapOf (mupdate i a t) j = ((mapOf t)(i |-> a)) j"
+  proof (cases "i = j")
+    case True 
+    then show ?thesis
+      using mapset_some setSpec upres vr by fastforce
+  next 
+    case False note i2nei = this
+    from i2nei have rhs_res: "((mapOf t)(i |-> a)) j = mapOf t j" by auto
+    have lhs_res: "mapOf (mupdate i a t) j = mapOf t j"
+    proof (cases "mapOf t j")
+      case None 
+      then show ?thesis
+        by (metis DiffD1 Un_empty_right Un_insert_right i2nei insertE mapset_none
+            prod.inject setSpec upres assms vr)
+    next 
+      case (Some z) 
+      then have mapSome: "mapOf t j = Some z" 
+        by simp
+      then have "(j,z) \<in> setOf t"
+        by (meson mapset_some assms)
+      with setSpec i2nei mapset_some vr have "mapOf ?tr j = Some z"
+        by (fastforce simp: eqs_def)
+      then show ?thesis
+        by (simp add: mapSome upres)
     qed
     from lhs_res rhs_res show ?thesis by simp
   qed
 qed
 
-lemma assumes v: "valid_tmap t"
-      shows mupdate_valid: "valid_tmap (mupdate i a t)"
-proof -
-  let ?tr = "binsert fst (i,a) t"
-  have upres: "mupdate i a t = ?tr" by (simp add: mupdate_def)
-  from v binsert_sorted have vr: "valid_tmap ?tr" by fastforce
-  from vr upres show ?thesis by simp
-qed
+lemma mupdate_valid: 
+  assumes "valid_tmap t" shows "valid_tmap (mupdate i a t)"
+  by (metis binsert_sorted mupdate_def assms valid_tmap_def)
 
 (*============================================================*)
 section \<open>Map Remove Operation\<close>
 (*============================================================*)
 
 definition mremove :: "index => 'a tarray => 'a tarray" where
-  "mremove i t == remove fst (i, undefined) t"
+  "mremove i t \<equiv> remove fst (i, undefined) t"
 
-lemma assumes v: "valid_tmap t"
-      shows mremove_valid: "valid_tmap (mremove i t)"
-proof (simp add: mremove_def)
-  from v remove_sort 
-  show "sortedTree fst (remove fst (i, undefined) t)" by fastforce
-qed
+lemma mremove_valid: 
+  assumes "valid_tmap t"
+  shows "valid_tmap (mremove i t)"
+  by (metis mremove_def remove_sort assms valid_tmap_def)
 
-lemma assumes v: "valid_tmap t"
-      shows mremove_map: "mapOf (mremove i t) i = None"
-proof (simp add: mremove_def)
-  let ?tr = "remove fst (i, undefined) t"
-  show "mapOf ?tr i = None"
-  proof -
-    from v remove_spec 
-    have remSet: "setOf ?tr = setOf t - eqs fst (i, undefined)"
-    by fastforce
-    have noneIn: "\<forall>a. (i,a) \<notin> setOf ?tr"
-    proof 
-      fix a
-      from remSet show "(i,a) ~: setOf ?tr" by (simp add: eqs_def)
-    qed
-    from v remove_sort have vr: "valid_tmap ?tr" by fastforce
-    have mapset_none_inst: "valid_tmap ?tr ==>
-    (mapOf ?tr i = None) = (\<forall>a. (i,a) \<notin> setOf ?tr)"
-    by (insert mapset_none [of "?tr" "i"], simp)
-    from vr this have "(mapOf ?tr i = None) = (\<forall>a. (i,a) \<notin> setOf ?tr)" by fastforce
-    from this noneIn show "mapOf ?tr i = None" by simp    
-  qed
-qed
+lemma mremove_map: 
+  assumes "valid_tmap t"
+  shows "mapOf (mremove i t) i = None"
+  using assms
+  by (auto simp: mremove_def eqs_def mapset_none remove_set remove_sort)
 
 end
